proof/security/FO_UU.ec
@@ -1,0 +1,1394 @@
+require import AllCore Distr List Real SmtMap FSet DInterval FinType KEM_ROM.
+require (****) PKE_ROM PlugAndPray Hybrid FelTactic. 
+
+(* This will be the underlying scheme resulting 
+   from the T transform, since we will need to
+   assume some of the properties that it offers.. *)
+require FO_TT.
+clone import FO_TT as TT.
+import PKE.
+
+(* we inherit the following axioms 
+dplaintext_ll: is_lossless dplaintext
+ dplaintext_uni: is_uniform dplaintext
+ dplaintext_fu: is_full dplaintext
+ FinT.enum_spec: forall (x : plaintext), count (pred1 x) enum = 1
+ kg_ll: is_lossless kg
+ randd_ll: is_lossless randd
+ ge0_qH: 0 <= qH
+ ge0_qV: 0 <= qV
+ ge0_qP: 0 <= qP
+ ge0_qHC: 0 <= qHC *)
+
+(* the type of KEM keys *)
+type key.
+op [lossless uniform full]dkey : key distr.
+
+(*  A PRF *)
+
+require PRF.
+print PRF.
+clone import PRF as J with
+   type D <- plaintext * ciphertext,
+   type R <- key.
+clone import RF with 
+   op dR <- fun _ => dkey
+   proof dR_ll by (move => *;apply dkey_ll)
+   proof *.
+(* we get the prf key type K from the next clone *)
+clone import PseudoRF.
+(**********)
+
+clone import KEM_ROM.KEM_ROM as KEMROM with
+   type pkey <- pkey,
+   type skey = (pkey * skey) * K,
+   type ciphertext <- ciphertext,
+   type key <- key,
+   op dkey <- dkey,
+   type RO.in_t <- plaintext,
+   type RO.out_t <- key,
+   op   RO.dout <- fun _ => dkey,
+   type RO.d_in_t <- unit, 
+   type RO.d_out_t <- bool
+   proof dkey_ll by apply dkey_ll
+   proof dkey_uni by apply dkey_uni
+   proof dkey_fu by apply dkey_fu
+   proof *.
+
+(******* Query Bounds ******)
+
+(* Max number of calls to RO in attack on UU *)  
+const qHU : { int | 0 <= qHU } as ge0_qHU. 
+(* Maximum number of calls to Dec on TT *) 
+const qD : { int | 0 <= qD } as ge0_qD.
+
+(***************************************)
+
+module (UU(HT : PKEROM.POracle) : KEMROM.Scheme) (HU : POracle) = {
+  proc kg() : pkey * skey = {
+     var pk, sk, k;
+     (pk,sk) <$ kg;
+     k <$ dK;
+     return (pk, ((pk,sk),k));
+  }
+  
+  proc enc(pk : pkey) : ciphertext * key = {
+     var m, c, k;
+     m <$ dplaintext;
+     c <@TT(HT).enc(pk,m);
+     k <@ HU.get(m);
+     return (c,k);
+  }
+  
+  proc dec(sk : skey, c : ciphertext) : key option = {
+     var m', k;
+     k <- witness;
+     m' <@ TT(HT).dec(sk.`1,c);
+     if (m' = None) {
+        k <- F sk.`2 (oget m', c);
+     }
+     else {
+        k <@ HU.get(oget m');
+     }
+     return (Some k);
+  }
+}.
+
+(* RO init must initialize both ROs *)
+
+module ROdI : KEMROM.Oracle = {
+   include KEMROM.RO.RO [-init]
+   proc init() : unit = {
+      PKEROM.RO.RO.init();
+      KEMROM.RO.RO.init();
+   }
+}.
+
+
+(* Correctness proof *)
+
+module (B_UC : PKEROM.CORR_ADV)  (HT : PKEROM.POracle)= {
+   proc find(pk : pkey, sk : PKEROM.skey) : plaintext = {
+      var m;
+      m <$ dplaintext;
+      return m;
+   }
+}.
+
+lemma correctness &m : 
+   Pr [ KEMROM.Correctness(ROdI,UU(PKEROM.RO.RO)).main() @ &m : res ] <=
+     Pr [ PKEROM.Correctness_Adv(PKEROM.RO.RO,TT,B_UC).main() @ &m : res ].
+proof.
+byequiv => //.
+proc.
+inline {1} 1; inline {1} 3; inline {1} 6. 
+inline {2} 2;inline {2} 4.
+seq 4 2 : (={PKEROM.RO.RO.m} /\ 
+            pk0{1} = kpair{2}.`1 /\ 
+            sk0{1} = kpair{2}.`2); 
+      1: by inline *;rnd{1};rnd;auto;smt(dK_ll).
+sp.
+seq 1 1 : (#pre /\ m{1} = m0{2}); 1: by auto.
+sp. 
+seq 2 1 : (#pre /\ c0{1} = c{2} /\ m{1} \in KEMROM.RO.RO.m{1} /\
+         k1{1} = oget KEMROM.RO.RO.m{1}.[m{1}]);1: 
+   by inline *;wp;rnd{1};wp;auto;smt(mem_set).
+inline {1} 2;sp.
+seq 1 1 : (#pre /\ m'{1} = m'{2}); 
+  1: by inline *;wp;conseq />;sim;auto => /#.
+by inline *;if{1};inline *;auto => />;smt(get_setE).
+qed.
+
+(* Security proof *)
+(*
+module CountO (O : VA_ORC) = {
+  var c_cvo : int
+  var c_pco : int
+  var c_h   : int
+  proc init () = { c_h <- 0; c_cvo <- 0; c_pco <- 0; }
+ 
+  proc cvo(c : ciphertext) : bool = {
+    var r;    
+    r <@ O.cvo(c);
+    c_cvo <- c_cvo + 1;
+    return r;
+  }
+  
+  proc pco(m : plaintext, c : ciphertext) : bool = {
+    var r;
+    r <@ O.pco(m, c);
+    c_pco <- c_pco + 1;
+    return r;
+  }
+}.
+
+module CountH(H:POracle) = {
+  proc get(x:plaintext) = {
+    var r;
+    r <@ H.get(x);
+    CountO.c_h <- CountO.c_h + 1;
+    return r;
+  }  
+}.
+
+module Gm = {
+  var m : plaintext
+  var r : randomness
+  var log : (plaintext, randomness) fmap
+  var bad_corr : plaintext option
+}.
+
+(* TODO : move this in SmtMap *)
+
+op find ['a, 'b] (f: 'a -> 'b -> bool) (m:('a, 'b) fmap) : ('a * 'b) option = 
+  let bindings = map (fun a => (a, oget m.[a])) (elems (fdom m)) in
+  let n = find (fun (p: _ * _) => f p.`1 p.`2) bindings in
+  if n < size bindings then Some (nth witness bindings n)
+  else None.
+
+lemma find_map ['a, 'b]:
+  forall (l : 'a list) (f : 'a -> 'b) (P : 'b -> bool),
+    find P (map f l) = find (fun (x : 'a) => P (f x)) l
+  by move => l f p; elim l;smt().
+
+lemma findP_Some ['a, 'b] (f: 'a -> 'b -> bool) (m:('a, 'b) fmap) a b: 
+  find f m = Some (a, b) =>
+  m.[a] = Some b /\ f a b by 
+   smt(mem_nth has_find find_ge0 List.mem_map fdomP mapP nth_find).
+
+lemma findP_None ['a, 'b] (f: 'a -> 'b -> bool) (m:('a, 'b) fmap): 
+  find f m = None =>
+  forall a b, m.[a] = Some b => !f a b
+ by smt(all_predC   has_find  List.mem_map fdomP mapP  allP).
+
+module O_AdvOW = {
+  var pk : pkey
+  proc pco(m : plaintext, c : ciphertext) : bool = {
+    var r, c';
+    r  <@ RO.RO.get(m);
+    c' <- enc r pk m;
+    return c = c';
+  }
+  
+  proc cvo(c:ciphertext) : bool = {
+    var rv; 
+    rv <- false; 
+    if (c <> OW_PCVA.cc) 
+      rv <- find (fun m r => c = enc r pk m) RO.RO.m <> None;
+    return rv;
+  }
+}.
+
+module AdvOW (A:PCVA_ADV) = {
+  import var OW_PCVA O_AdvOW
+
+  module A = A(CountH(RO.RO), CountO(O_AdvOW))
+
+  proc find(pk0:pkey, c:ciphertext) : plaintext = {
+    var m' : plaintext;
+    pk <- pk0; 
+    RO.RO.init();
+    cc       <- c; 
+    CountO(O_AdvOW).init();
+    m'       <@ A.find(pk,cc);
+    return m'; 
+  }
+}.
+
+module AdvOW_query (A:PCVA_ADV) = {
+  import var OW_PCVA O_AdvOW
+
+  module A = A(CountH(RO.RO), CountO(O_AdvOW))
+
+  proc main(pk0:pkey, c:ciphertext) : unit = {
+    var m' : plaintext;
+    pk <- pk0; 
+    RO.RO.init();
+    cc       <- c; 
+    CountO(O_AdvOW).init();
+    m'       <@ A.find(pk,cc);
+  }
+
+  proc find(pk0:pkey, c:ciphertext) : plaintext = {
+    var i : int;
+    main(pk0, c);
+    i        <$ [0 .. qH + qP - 1];
+    return nth witness (elems (fdom RO.RO.m)) i;
+  }
+}.
+
+section. 
+
+declare module A <: PCVA_ADV { -OW_PCVA, -RO.RO, -RO.FRO, -CountO, -Gm, -O_AdvOW, -Correctness_Adv1, -B}.
+
+local module PCO(RO:RO.RO) = {
+  import var OW_PCVA
+  proc pco(m : plaintext, c : ciphertext) : bool = {
+    var m', rv, r, c';
+    rv <- false;
+    m' <- dec (sk.`2) c;
+    if (m' <> None) {
+      if (m' = Some m) {
+        r  <@ RO.get(m);
+        c' <- enc r sk.`1 m;
+        rv <- c = c';
+      } else {
+        RO.sample(m);
+        r <@ RO.get(oget m');  
+      }      
+    } else RO.sample(m);
+    return rv;
+  }   
+}.
+
+(* local *) module type PCOT = {
+  proc pco(m : plaintext, c:ciphertext) : bool
+}.
+
+(* local *) module type GT (PCO:PCOT) (RO:RO.RO) = {
+  proc distinguish () : bool
+}.
+
+local module G (PCO:PCOT) (RO:RO.RO) = {
+  import var OW_PCVA
+
+  module O = {
+    proc pco = PCO.pco
+
+    proc cvo(c:ciphertext) : bool = {
+      var m : plaintext option;
+      m <- None;
+      if (c <> cc) m <@ TT(RO).dec(sk, c); 
+      return (m <> None);
+    }
+  }
+
+  module A = A(RO,O)
+
+  proc distinguish() : bool = {
+    var pk : pkey;
+    var r : randomness;
+    var m, m' : plaintext;
+    var b;
+    RO.init();
+    (pk, sk) <@ TT(RO).kg();
+    m        <$ dplaintext;
+    r        <@ RO.get(m);
+    cc       <- enc r pk m; 
+    m'       <@ A.find(pk,cc);
+    b        <- dec sk.`2 cc = Some m';
+    return b; 
+  }
+}.
+
+local module G_PCO (RO:RO.RO) = G(PCO(RO), RO).
+
+import RO.FullEager.
+
+(* Generalize means that, to win the OW game, 
+   one does not need to actually find a message 
+   for which TT passes the check, but merely
+   solve the owness of the underlying pke *)
+local lemma OW_PCVA_G_PCO &m : 
+  Pr[OW_PCVA(RO.LRO, TT, A).main() @ &m : res] <= 
+        Pr[G_PCO(RO.LRO).distinguish() @ &m : res].
+proof.
+  byequiv => //; proc.
+  seq 5 6: (={m', glob OW_PCVA}).
+  + call (: ={glob RO.RO, glob OW_PCVA}).
+    + by sim.
+    + proc; inline{1} 1; sp; wp.
+      if => //; 2: by inline *; auto.
+      if{2}.
+      + wp; call (: ={glob RO.RO}); 1: by sim.     
+        by skip => /> /#.
+      wp; call (: ={glob RO.RO}); 1: by sim. 
+      by inline *; auto => /> /#.
+    + by sim.
+    inline{1} 4; wp.
+    call (: ={glob RO.RO}); 1: by sim.
+    by inline *; auto.
+  inline{1} 1; inline{1} 3; sp; wp.
+  if{1}; 2: by auto => /> ? ->.
+  wp; call{1} (: true ==> true); 1: by islossless.
+  by skip => /> /#.
+qed.
+
+local module PCO1(RO:RO.RO) = {
+  import var OW_PCVA
+  proc pco(m : plaintext, c : ciphertext) : bool = {
+    var m', rv, r, c';
+    rv <- false;
+    m' <- dec (sk.`2) c;
+    if (m' <> None) {
+      if (m' = Some m) {
+        r  <@ RO.get(m);
+        c' <- enc r sk.`1 m;
+        rv <- c = c';
+      } else {
+        r <@ RO.get(m);
+        RO.sample(oget m');  
+      }      
+    } else r <@ RO.get(m);
+    return rv;
+  }   
+}.
+
+local module G_PCO1 (RO:RO.RO) = G(PCO1(RO), RO).
+
+local module PCO2(RO:RO.RO) = {
+  import var OW_PCVA
+  proc pco(m : plaintext, c : ciphertext) : bool = {
+    var m', rv, r, c';
+    rv <- false;
+    m' <- dec (sk.`2) c;
+    r  <@ RO.get(m);
+    if (m' = Some m) {
+        c' <- enc r sk.`1 m;
+        rv <- c = c';
+    }
+    return rv;
+  }   
+}.
+
+local module G_PCO2 = G(PCO2(RO.RO), RO.RO).
+
+(* abstracting over G and making sure m is always in the rom table for PCO2 queries.
+   It might not be if the ciphertext failed to decrypt. *)
+local lemma PCO_PCO2 &m : 
+   Pr[G_PCO (RO.LRO).distinguish() @ &m : res] =
+   Pr[G_PCO2.distinguish() @ &m : res].
+proof.
+  have hll : forall (_ : plaintext), is_lossless randd by move=> _; apply randd_ll.
+  have <- : Pr[G_PCO(RO.RO).distinguish() @ &m : res] =
+            Pr[G_PCO(RO.LRO).distinguish() @ &m : res]. 
+  + by byequiv (RO.FullEager.RO_LRO_D (<:G_PCO) hll).
+  have -> : Pr[G_PCO (RO.RO).distinguish() @ &m : res] = 
+            Pr[G_PCO1(RO.RO).distinguish() @ &m : res].
+  + byequiv => //.
+    sim (G_PCO(RO.RO).O.pco ~ G_PCO1(RO.RO).O.pco : ={glob RO.RO, glob OW_PCVA}).
+    proc; sp; if => //. 
+    + if => //; 1: by sim.
+      call (: ={x, glob RO.RO} ==> ={glob RO.RO});1: by proc; inline *; sim.
+      call (: ={x, glob RO.RO} ==> ={glob RO.RO});1: by proc; inline *; sim.
+      by auto.
+    call (: ={x, glob RO.RO} ==> ={glob RO.RO});1: by proc; inline *; sim.
+    by auto.
+  have -> : Pr[G_PCO1(RO.RO).distinguish() @ &m : res] =
+            Pr[G_PCO1(RO.LRO).distinguish() @ &m : res].
+  + by byequiv (RO.FullEager.RO_LRO_D (<:G_PCO1) hll).
+  byequiv => //.
+  sim (G_PCO1(RO.LRO).O.pco ~ G_PCO2.O.pco : ={glob RO.RO, glob OW_PCVA}).
+  proc; sp.
+  if{1}; last first.
+  + rcondf{2} ^if; 2: by sim. 
+    by move=> *; conseq (: true) => /> // ->.
+  if{1}.
+  + rcondt{2} ^if; 2: by sim.
+    by move=> *; conseq (:true) => />.
+  rcondf{2} ^if; 1: by move=> *; conseq (:true) => />.
+  by inline{1} 2; wp; sim.
+qed.
+
+local clone import Hybrid as Hybrid0 with 
+type input    <- plaintext * skey * ciphertext,
+type output   <- bool,
+type inleaks  = plaintext option,
+type outleaks = randomness option,
+type outputA <- bool,
+op q  <- qV
+proof q_ge0 by smt(ge0_qV) 
+proof *. (* This line allow to be sure that no remaining axiom are still present *)
+
+local module Orclb_ (RO:RO.RO) : Orclb = {
+
+  proc leaks (il : inleaks) : outleaks = {
+    var re, r; 
+
+    if (il = None) { 
+      RO.init(); 
+      re <- None; }
+    else {
+      r <@ RO.get (oget il);
+      re <- Some r;
+    }
+    return re;
+  }
+
+  proc orclR (m:plaintext, sk: skey, c:ciphertext) : bool = {
+    return false;
+  }
+
+  proc orclL (m:plaintext, sk: skey, c:ciphertext) : bool = {
+    var r, c', rv;
+    r <@ RO.get(m);
+    c' <- enc r (sk.`1) (m);
+    rv <- c = c';
+    return rv;
+  }
+}.
+
+local module Orclb = Orclb_(RO.RO).
+
+module H(RO:POracle) = { 
+  import var Gm
+  proc get (x:plaintext) = {
+    var r;
+    if (x \notin log) {
+      r <@ RO.get(x);
+      log.[x] <- r;
+    }
+    return oget log.[x];
+  }
+}.
+
+(* Jumps to a game where the ciphertext validity oracle
+   cannot possibly interfere with OW solutions because
+   it will reject all entries that encrypt the challenge
+   m. This is done one cvo query at a time *)
+local module G0 (Ob:Orclb) (Oh:Orcl) = {
+  import var OW_PCVA Gm
+
+  module RO = {
+    proc init () = {Ob.leaks(None); log <- empty; }
+    proc get (m:plaintext) = { var r; r <@ Ob.leaks(Some m); return oget r; }
+  }
+
+  module H = H(RO)
+
+  module O = {
+    proc pco(m : plaintext, c : ciphertext) : bool = {
+      var m', rv, r, c';
+      rv <- false;
+      m' <- dec (sk.`2) c;
+      r  <@ H.get(m);
+      if (m' = Some m) {
+        c' <- enc r sk.`1 m;
+        rv <- c = c';
+      }
+      return rv;
+    }
+
+    proc cvo(c:ciphertext) : bool = {
+      var rv, m', r, c';
+
+      rv <- false; 
+      if (c <> cc) { 
+        m' <- dec (sk.`2) c;
+        if (m' <> None) {
+          if (oget m' \in log) { 
+            r   <- oget log.[oget m']; 
+            c' <- enc r (sk.`1) (oget m');
+            rv <- c = c';
+          } else {
+            if (oget m' = Gm.m) {
+              c' <- enc Gm.r (sk.`1) (oget m');
+              rv <- c = c';
+            } else rv <@ Oh.orcl(oget m', sk, c);
+          }
+        }
+      }
+      return rv;
+    }
+  }
+
+  module A = A(CountH(H), CountO(O)) 
+
+  proc main() : bool = {
+    var pk : pkey;
+    var m' : plaintext;
+    var b;
+    RO.init();
+    (pk, sk) <@ TT(RO).kg();
+    m        <$ dplaintext;
+    r        <@ RO.get(m);
+    cc       <- enc r pk m; 
+
+    CountO(O).init();
+    m'       <@ A.find(pk,cc);
+    b        <- dec sk.`2 cc = Some m';
+    return b; 
+  }
+
+}.
+
+op incl ['a, 'b] (m1 m2: ('a, 'b) fmap) = 
+  forall x, x \in m1 => m1.[x] = m2.[x].
+
+local equiv RO_get : RO.RO.get ~ RO.RO.get : 
+  ={arg} /\ (={glob RO.RO} /\ (incl Gm.log RO.RO.m /\ RO.RO.m.[Gm.m] = Some Gm.r){2}) 
+  ==>
+  ={res} /\ (={glob RO.RO} /\ (incl Gm.log RO.RO.m /\ RO.RO.m.[Gm.m] = Some Gm.r){2}).
+proof.
+  proc; inline *; auto => />; smt (get_setE).
+qed.
+
+local equiv RO_RO0_get : RO.RO.get ~ G0(Orclb, OrclCount(L(Orclb))).RO.get : 
+  ={arg} /\ (={glob RO.RO} /\ (incl Gm.log RO.RO.m /\ RO.RO.m.[Gm.m] = Some Gm.r){2}) 
+  ==>
+  ={res} /\ (={glob RO.RO} /\ (incl Gm.log RO.RO.m /\ RO.RO.m.[Gm.m] = Some Gm.r){2}).
+proof.
+  proc; inline *; rcondf{2} 2; auto => />; smt (get_setE).
+qed.
+
+local equiv RO_H_get : RO.RO.get ~ G0(Orclb, OrclCount(L(Orclb))).H.get : 
+  ={arg} /\ (={glob RO.RO} /\ (incl Gm.log RO.RO.m /\ RO.RO.m.[Gm.m] = Some Gm.r){2}) 
+  ==>
+  ={res} /\ (={glob RO.RO} /\ (incl Gm.log RO.RO.m /\ RO.RO.m.[Gm.m] = Some Gm.r){2}).
+proof.
+  proc *; inline *; wp; sp.
+  if{2}; 1: rcondf{2} 3; auto => />; smt(get_setE).
+qed.
+
+local lemma G_PCO2_G0 &m : 
+  Pr[G_PCO2.distinguish() @ &m : res] = Pr[Ln(Orclb,G0).main() @ &m : res].
+proof.
+  byequiv ( : ={glob A} ==> ={res}) => //.
+  proc; inline{2} 2; wp.
+  call (: ={glob OW_PCVA, glob RO.RO} /\ (incl Gm.log RO.RO.m /\ RO.RO.m.[Gm.m] = Some Gm.r){2}).
+  + proc. inline TT(RO.RO).dec; inline{2} 1; wp; sp; if => //.
+    wp; sp; if => //.
+    if{2}; 1 : by inline *; auto => /> /#.
+    inline OrclCount(L(Orclb)).orcl Count.incr L(Orclb).orcl.
+    if{2}.
+    + by inline{1} 1; rcondf{1} ^if; auto => /> /#.
+    by wp; call RO_get; auto => /> /#.
+  + proc *. inline{2} 1; wp.
+    inline{1} 1; inline{2} 3.
+    by wp; call RO_H_get; wp; skip => /> /#.
+  + by proc *; inline{2} 1; wp; call RO_H_get; auto.
+  inline{2} 7; wp.
+  inline *.
+  rcondt{1} ^if; 1: by auto; move=> *; rewrite mem_empty.
+  rcondt{2} 3; 1: by auto.
+  rcondf{2} ^if; 1: by auto.
+  rcondt{2} ^if; 1: by auto; move=> *; rewrite mem_empty.
+  auto => />; smt(get_setE mem_empty).
+qed.  
+
+(* Remark : Rn(Orclb,HA).main corresponds to game G1 in HHK *)
+
+local lemma G0_G1 &m : 
+ (forall (RO<:POracle{ -CountO, -A })(O<:VA_ORC { -CountO, -A }), 
+  hoare [A(CountH(RO), CountO(O)).find : 
+       CountO.c_h = 0   /\ CountO.c_cvo = 0   /\ CountO.c_pco = 0 ==> 
+       CountO.c_h <= qH /\ CountO.c_cvo <= qV /\ CountO.c_pco <= qP]) =>
+
+  (forall (H0 <: POracle { -A }) (O <: VA_ORC { -A }),
+  islossless O.cvo => islossless O.pco => islossless H0.get => islossless A(H0, O).find) =>
+
+  Pr[Ln(Orclb,G0).main() @ &m : res] =
+  Pr[Rn(Orclb,G0).main() @ &m : res] +
+    qV%r * (Pr[HybGame(G0,Orclb,L(Orclb)).main() @ &m : res]
+               - Pr[HybGame(G0,Orclb,R(Orclb)).main() @ &m : res]).
+proof.
+  move => A_count A_ll.
+  have /= /# := Hybrid_restr Orclb G0 _ _ _ _ _ &m (fun _ _ _ r => r).
+  + move=> O.
+    proc. inline 2.
+    conseq (_ : Count.c <= CountO.c_cvo) (_: CountO.c_cvo <= qV); 1: smt().
+    + wp; call (A_count (<:G0(Orclb, OrclCount(O)).H) (<: G0(Orclb, OrclCount(O)).O)).
+      by inline 7; wp; conseq />.
+    wp; call (: Count.c <= CountO.c_cvo).
+    + proc; inline 1; wp; sp.
+      if; 2: skip => /#.
+      sp; if; 2: skip => /#.
+      if; 1: auto => /> /#.
+      if; 1: auto => /> /#.
+      inline 1; inline 3; wp.
+      by conseq (: true) => // /#.
+    + by conseq />.
+    + by conseq />.
+    by inline 7; wp; inline 1; sp; conseq />.
+  + by islossless. + by islossless. + by islossless.
+  move=> Ob0 LR orcl_ll leaks_ll orclL_ll orclR_ll.
+  islossless; apply (A_ll (<:CountH(G0(Ob0, LR).H)) (<:CountO(G0(Ob0, LR).O))); islossless.
+qed.
+
+(* We bound the diff between the HybGame *)
+local module Orclb1 : Orclb = {
+  var bad : bool
+  include var Orclb[leaks, orclL]
+
+  proc orclR (m:plaintext, sk: skey, c:ciphertext) : bool = {
+    var r;
+    r <@ RO.RO.get(m);
+    bad <- bad || enc r (sk.`1) (m) = c;
+    return false;
+  }
+}.
+
+local module Orclb2(RO:RO.RO) : Orclb = {
+  include var Orclb_(RO)[leaks, orclL]
+
+  proc orclR (m:plaintext, sk: skey, c:ciphertext) : bool = {
+    RO.sample(m);
+    return false;
+  }
+}.
+
+(* Abstracting over HybGame(G0) *)
+
+local module H_bad_ (HA: AdvOrclb)(O:Orclb) = {
+   var c : int
+   proc main () = {
+     var b;
+     Orclb1.bad <- false; c <- 0;
+     b <@ HA(Orclb,R(O)).main();
+     return b;
+   }
+}.
+
+local module H_bad (HA:AdvOrclb) = H_bad_ (HA, Orclb1).
+
+local module D (HA:AdvOrclb) (RO:RO.RO) = {
+  proc distinguish = HA(Orclb_(RO),R(Orclb2(RO))).main
+}.
+
+local lemma HA_bad1 (HA <: AdvOrclb {-Orclb, -Orclb1, -RO.FRO, -H_bad}) &m : 
+  ( forall (Ob <: Orclb{-HA}) (O <: Orcl{-HA}),
+     islossless O.orcl => islossless Ob.leaks => islossless Ob.orclL => islossless Ob.orclR => 
+     islossless HA(Ob, O).main) =>
+   Pr[HA(Orclb,L(Orclb)).main() @ &m : res] <=
+   Pr[HA(Orclb,R(Orclb)).main() @ &m : res] + 
+   Pr[H_bad(HA).main() @ &m : Orclb1.bad].
+proof.
+  move=> HA_ll.
+  have <- :  
+    Pr[H_bad(HA).main() @ &m : res] = 
+    Pr[HA(Orclb,R(Orclb)).main() @ &m : res].
+  (* We need lazy/eager *)
+  + have -> : 
+      Pr[H_bad(HA).main() @ &m : res] = 
+      Pr[D(HA, RO.RO).distinguish() @ &m : res].
+    + byequiv => //. 
+      proc *; inline{1} 1; wp. 
+      sim (Orclb1.orclR ~ Orclb2(RO.RO).orclR : ={RO.RO.m}).
+      by proc; inline *; sim.
+    have -> : Pr[D(HA, RO.RO).distinguish() @ &m : res] =
+              Pr[D(HA, RO.LRO).distinguish() @ &m : res].
+    + by byequiv(RO_LRO_D (D(HA)) _) => // *; apply randd_ll.
+    byequiv => //.
+    sim (: ={glob RO.RO}).
+    by proc; inline *; auto.
+  byequiv => //.
+  proc *; inline{2} 1.
+  wp; call (: Orclb1.bad, ={glob Orclb}).
+  + proc.
+    wp; call (: ={glob RO.RO}); 1: by sim.
+    auto => /> /#.
+  + by move=> *; islossless.
+  + move=> *; proc; wp; conseq (_: true) => />; islossless.
+  + by sim />.
+  + by move=> *; islossless.
+  + by move=> *; conseq />; islossless.
+  + by conseq (: ={res, glob Orclb}) => //; sim.
+  + by move=> *; islossless.
+  + by move=> *; conseq />; islossless.
+  + by conseq (: ={res, glob Orclb}) => //; sim.
+  + by move=> *; islossless.
+  + by move=> *; conseq />; islossless.
+  by auto => /> /#.
+qed.
+
+local lemma G0_G1_1 &m : 
+ (forall (RO<:POracle{ -CountO, -A })(O<:VA_ORC { -CountO, -A }), 
+  hoare [A(CountH(RO), CountO(O)).find : 
+       CountO.c_h = 0   /\ CountO.c_cvo = 0   /\ CountO.c_pco = 0 ==> 
+       CountO.c_h <= qH /\ CountO.c_cvo <= qV /\ CountO.c_pco <= qP]) =>
+
+  (forall (H0 <: POracle { -A }) (O <: VA_ORC { -A }),
+  islossless O.cvo => islossless O.pco => islossless H0.get => islossless A(H0, O).find) =>
+  Pr[Ln(Orclb,G0).main() @ &m : res] <=
+  Pr[Rn(Orclb,G0).main() @ &m : res] + 
+    qV%r * Pr[H_bad(HybGame(G0)).main() @ &m : Orclb1.bad].
+proof.
+  move => A_count A_ll.
+  have -> := G0_G1 &m A_count A_ll.
+  case(qV = 0);1: by smt().
+  move => qVn0.
+  apply StdOrder.RealOrder.ler_add => //.
+  apply StdOrder.RealOrder.ler_pmul2l; 1: smt (ge0_qV).
+  have /# := HA_bad1 (HybGame(G0)) &m _.
+  move=> Ob O orcl_ll leaks_ll orclL_ll orclR_ll; islossless.
+  + apply (A_ll (<:CountH(G0(Ob, HybOrcl(Ob, O)).H)) (<:CountO(G0(Ob, HybOrcl(Ob, O)).O))); islossless.
+  smt (dinter_ll ge0_qV).
+qed.
+
+(* Now we focus on 
+     Pr[H_bad(HybGame(G0)).main() @ &m : Orclb1.bad]
+   We show that it is less than gamma_spread.
+   Remark that bad can be set only once ...
+*)
+
+local module Orclb1' : Orclb = {
+  include var Orclb[leaks, orclL]
+  import var Orclb1
+
+  proc orclR (m:plaintext, sk: skey, c:ciphertext) : bool = {
+    var r;
+    (* This test is added for the next step, it ensure that sk in a valid key pair *)
+    if (sk \in kg) { 
+      r <$ randd;
+      RO.RO.m.[m] <- r;
+      bad <- bad || enc r (sk.`1) (m) = c;
+    }
+    H_bad_.c <- H_bad_.c + 1;
+    return false;
+  }
+}.
+
+local equiv Orclb1_Orclb1'_Hget : 
+  G0(Orclb, HybOrcl(Orclb, R(Orclb1))).H.get ~
+  G0(Orclb, HybOrcl(Orclb, R(Orclb1'))).H.get : 
+  ={arg} /\ (={glob RO.RO, glob OW_PCVA, glob Orclb1, Gm.log, Gm.m, Gm.r, glob HybOrcl} /\
+            (HybOrcl.l <= HybOrcl.l0 => eq_except (pred1 Gm.m) Gm.log RO.RO.m){2}) ==>
+  ={res} /\ (={glob RO.RO, glob OW_PCVA, glob Orclb1, Gm.log, Gm.m, Gm.r, glob HybOrcl} /\
+            (HybOrcl.l <= HybOrcl.l0 => eq_except (pred1 Gm.m) Gm.log RO.RO.m){2}).
+proof.
+  proc; if => //; inline *; wp.
+  rcondf{1} ^if; 1: by auto.
+  rcondf{2} ^if; 1: by auto.
+  auto => />; smt (get_setE).
+qed.
+
+local lemma H_bad_Orclb1' &m : 
+  Pr[H_bad(HybGame(G0)).main() @ &m : Orclb1.bad] = 
+  Pr[H_bad_(HybGame(G0), Orclb1').main() @ &m : Orclb1.bad /\ H_bad_.c <= 1].
+proof.
+  byequiv => //; proc.
+  inline{1} 3; inline{2} 3.
+  inline{1} 5; inline{2} 5.
+  wp. 
+  call ( : ={glob RO.RO, glob OW_PCVA, glob Orclb1, Gm.log, Gm.m, Gm.r, glob HybOrcl} /\
+            (H_bad_.c = b2i (HybOrcl.l0 < HybOrcl.l)){2} /\
+            (OW_PCVA.sk \in kg){2} /\
+            (HybOrcl.l <= HybOrcl.l0 => eq_except (pred1 Gm.m) Gm.log RO.RO.m){2}).
+  + proc; wp; inline{1} 1; inline{2} 1; sp; wp.
+    if => //; sp; if => //.
+    if => //; 1: by auto.
+    if => //; 1: by auto.
+    inline{1} 1; inline{2} 1; sp; wp.
+    if => //; 1: by inline *; auto => />; smt(get_setE).
+    if => //; 2: by inline *; auto => /> /#.
+    inline *; rcondt{1} ^if; 1: by auto => /> /#.
+    by rcondt{2} ^if; auto => />; smt(get_setE).
+  + proc; wp.
+    inline{1} 1; inline{2} 1.
+    by wp; call Orclb1_Orclb1'_Hget; wp. 
+  + by proc; wp; call Orclb1_Orclb1'_Hget.
+  inline *.
+  rcondt{1} 6; 1: by auto.
+  rcondt{2} 6; 1: by auto.
+  rcondf{1} ^if; 1: by auto.
+  rcondf{2} ^if; 1: by auto.
+  auto => />; smt(get_setE mem_empty supp_dinter).
+qed.
+
+pred gamma_spread_ok(gamma_spread : real) = 
+ forall pk sk m c, (pk, sk) \in kg =>
+   mu randd (fun r => enc r pk m = c) <= gamma_spread.
+
+local lemma ge0_gamma_spread gamma_spread :
+  gamma_spread_ok gamma_spread => 0%r <= gamma_spread.
+proof.
+rewrite /gamma_spread_ok => gOK.
+have := witness_support predT kg; rewrite kg_ll /= => pkskH.
+have := witness_support predT randd; rewrite randd_ll /= => rH.
+elim pkskH => pksk pkskin. 
+elim rH => r rin. 
+have :=  gOK pksk.`1 pksk.`2 witness (enc r pksk.`1 witness) _;1 :by smt().
+by smt(witness_support).
+qed.
+
+(* Now we can trivially bound the probability of Orcl1.bad using fel *)
+local lemma H_bad_gamma_spread &m gamma_spread: 
+  gamma_spread_ok gamma_spread => 
+  Pr[H_bad_(HybGame(G0), Orclb1').main() @ &m : Orclb1.bad /\ H_bad_.c <= 1] <=
+    gamma_spread.
+proof.
+  rewrite /gamma_spread_ok;move => gs_ok.
+  fel 2 H_bad_.c (fun _, gamma_spread) 1 Orclb1.bad []=> //.
+  + by rewrite StdBigop.Bigreal.BRA.big_int1.
+  + by auto.
+  + proc; wp; if; wp.
+    + rnd; skip => /> &1 _ _ _; case: (sk{1}) => pk sk hsk.
+      by apply (gs_ok pk sk m{1} c{1} hsk).
+    conseq (: _ ==> false : = 0%r) => />; 2: by auto.
+    by move=> &1 _ _ _ _; apply (ge0_gamma_spread gamma_spread gs_ok).
+  move=> c; proc; if; auto => /> /#.
+qed.
+
+local lemma OW_PCVA_gamma &m gamma_spread:
+ gamma_spread_ok gamma_spread =>
+ 
+ (forall (RO<:POracle{ -CountO, -A })(O<:VA_ORC { -CountO, -A }), 
+  hoare [A(CountH(RO), CountO(O)).find : 
+       CountO.c_h = 0   /\ CountO.c_cvo = 0   /\ CountO.c_pco = 0 ==> 
+       CountO.c_h <= qH /\ CountO.c_cvo <= qV /\ CountO.c_pco <= qP]) =>
+
+  (forall (H0 <: POracle { -A }) (O <: VA_ORC { -A }),
+  islossless O.cvo => islossless O.pco => islossless H0.get => islossless A(H0, O).find) =>
+
+  Pr[OW_PCVA(RO.LRO, TT, A).main() @ &m : res] <= 
+     Pr[Rn(Orclb,G0).main() @ &m : res] + qV%r * gamma_spread.
+proof.
+  move => gs_ok A_count A_ll.
+  have := (OW_PCVA_G_PCO &m).
+  rewrite (PCO_PCO2 &m) (G_PCO2_G0 &m).
+  move: (G0_G1_1 &m A_count A_ll) (H_bad_Orclb1' &m) (H_bad_gamma_spread &m) ge0_qV. 
+  by smt().
+qed.
+
+module G2_O (RO:POracle) = {
+  import var OW_PCVA Gm
+
+  proc pco(m : plaintext, c : ciphertext) : bool = {
+    var m', r, c';
+    m' <- dec (sk.`2) c;
+    r  <@ H(RO).get(m);
+    c' <- enc r sk.`1 m;
+    bad_corr <- if (c = c' /\ m' <> Some m) then Some m else bad_corr;
+    return c = c';
+  }
+  
+  proc cvo(c:ciphertext) : bool = {
+    var rv, m' (* , r, c' *);
+  
+    rv <- false; 
+    if (c <> cc) { 
+      m' <- dec (sk.`2) c;
+      rv <- find (fun m r => c = enc r sk.`1 m) log <> None;
+      if (m' <> None) {
+        if (oget m' \in log) { 
+           bad_corr <- 
+            let f = find (fun m r => c = enc r sk.`1 m) log in
+            if f <> None /\ (oget f).`1 <> oget m' then Some (oget f).`1 else bad_corr; 
+        } else {
+          if (oget m' = Gm.m) {
+            bad_corr <- 
+              let f = find (fun m r => c = enc r sk.`1 m) log in
+               if f <> None /\ (oget f).`1 <> oget m' then Some (oget f).`1 else bad_corr; 
+          } else {
+            bad_corr <- 
+              let f = find (fun m r => c = enc r sk.`1 m) log in
+              if f <> None then Some (oget f).`1 else bad_corr;
+          }
+        }    
+      } else {
+        bad_corr <- 
+          let f = find (fun m r => c = enc r sk.`1 m) log in
+          if f <> None then Some (oget f).`1 else bad_corr;
+      }
+    }
+    return rv;
+  }
+}.
+
+local module G2 = {
+  import var OW_PCVA Gm
+
+  module H = H(RO.RO)
+  module O = G2_O(RO.RO)
+  module A = A(CountH(H), CountO(O))
+
+  proc main() : bool = {
+    var pk : pkey;
+    var m' : plaintext;
+    var b;
+    RO.RO.init(); Gm.log <- empty; bad_corr <- None;
+    (pk, sk) <@ TT(RO.RO).kg();
+    m        <$ dplaintext;
+    r        <@ RO.RO.get(m);
+    cc       <- enc r pk m; 
+
+    CountO(O).init();
+    m'       <@ A.find(pk,cc);
+    b        <- dec sk.`2 cc = Some m' /\ m = m';
+    bad_corr <- if dec sk.`2 cc = Some m' /\ m <> m' then Some m else bad_corr;
+    return b; 
+  }
+
+}.
+
+local equiv G1_G2_RO : 
+  G0(Orclb_(RO.RO), OrclCount(R(Orclb_(RO.RO)))).RO.get ~ RO.RO.get : 
+  ={arg, glob RO.RO}
+  ==>
+  ={res, glob RO.RO}.
+proof.
+  proc; inline{1} 1; rcondf{1} 2; 1: by auto.
+  inline{1} 2; auto.
+qed.
+
+local equiv G1_G2_H : 
+  G0(Orclb_(RO.RO), OrclCount(R(Orclb_(RO.RO)))).H.get ~ G2.H.get : 
+  ={x, glob RO.RO, Gm.log}
+  ==>
+  ={res, glob RO.RO, Gm.log}.
+proof. by proc; if => //; wp; call G1_G2_RO. qed.
+ 
+local lemma G1_G2 &m : 
+  (forall (H0 <: POracle { -A }) (O <: VA_ORC { -A }),
+  islossless O.cvo => islossless O.pco => islossless H0.get => islossless A(H0, O).find) =>
+
+  Pr[Rn(Orclb,G0).main() @ &m : res] <= Pr[ G2.main() @ &m : res] + Pr[G2.main() @ &m : Gm.bad_corr <> None].
+proof.
+  move => A_ll.
+  byequiv => //; proc.
+  inline{1} 2; wp.
+  call (: Gm.bad_corr <> None, ={glob OW_PCVA, glob RO.RO, Gm.log, Gm.m, Gm.r} /\
+                          (OW_PCVA.cc = enc Gm.r OW_PCVA.sk.`1 Gm.m){2}).
+  + proc; wp.
+    inline{1} 1; inline{2} 1; sp 2 2.    
+    if => //; 2: by auto.
+    sp 1 2; if => //; 2: by wp; skip => /> &2; case: (find _ _).
+    if => //; 1: by auto => />; smt(findP_Some findP_None).
+    elim * => rv_R; inline *.  
+    by if => //; wp; skip => />; smt(findP_Some).
+  + by move=> *; islossless.
+  + by move=> _; proc; inline 1; wp; skip => /#.
+  + proc; wp; inline{1} 1; inline{2} 1.
+    by sp; wp; call G1_G2_H; skip => /> /#.
+  + by move=> *; islossless.
+  + move=> _; proc; inline 1; wp.
+    by conseq (: true); [smt() | islossless].
+  + by proc; wp; call G1_G2_H.
+  + by move=> *; islossless.
+  + by move=> *; conseq />; islossless.
+  inline{1} 7; inline{2} 8; wp.
+  call G1_G2_RO; inline *.
+  by rcondt{1} ^if; auto => /> /#.
+qed.
+
+module AdvCorr (A:PCVA_ADV) (RO:POracle) = {
+  import var OW_PCVA Gm
+
+  module H = H(RO)
+  module O = G2_O(RO)
+  module A = A(CountH(H), CountO(O))
+
+  proc find(pk:pkey, sk:skey) : plaintext = {
+    var m' : plaintext;
+    OW_PCVA.sk <- sk;
+    Gm.log <- empty; bad_corr <- None;
+    m        <$ dplaintext;
+    r        <@ RO.get(m);
+    cc       <- enc r pk m; 
+
+    CountO(O).init();
+    m'       <@ A.find(pk,cc);
+    bad_corr <- if dec sk.`2 cc = Some m' /\ m <> m' then Some m else bad_corr;
+    return oget Gm.bad_corr; 
+  }
+}.
+
+op inv_G2_corr (log ro : (plaintext, randomness) fmap) (sk:skey) 
+        bad_corr gm gr = 
+  incl log ro /\ gm \in ro /\ gr = oget ro.[gm] /\
+  (bad_corr <> None => 
+      let m = oget bad_corr in
+      let r = oget ro.[m] in
+      let c = enc r sk.`1 m in
+      let m' = dec sk.`2 c in
+      m \in ro /\ m' <> Some m).
+
+local equiv G2_corr_H m_ : H(RO.RO).get ~ H(RO.RO).get : 
+   ={x} /\ x{2} = m_ /\ ={glob RO.RO, glob Gm, glob OW_PCVA} /\ 
+   (inv_G2_corr Gm.log RO.RO.m OW_PCVA.sk Gm.bad_corr Gm.m Gm.r){2} ==>
+   ={res} /\  ={glob RO.RO, glob Gm, glob OW_PCVA} /\ 
+   ( m_ \in RO.RO.m /\ res = oget RO.RO.m.[m_] /\
+     inv_G2_corr Gm.log RO.RO.m OW_PCVA.sk Gm.bad_corr Gm.m Gm.r){2}.
+proof.
+  proc; if => //; 2: by skip => /> /#.
+  inline *; auto => />; smt(get_setE).
+qed.
+    
+local lemma G2_correctness &m : 
+  Pr[G2.main() @ &m : Gm.bad_corr <> None] <= 
+  Pr[ Correctness_Adv(RO.RO,TT,AdvCorr(A)).main() @ &m : res ].
+proof.
+  byequiv => //; proc.
+  inline{2} 3.
+  seq 11 13 : 
+    (={glob RO.RO, glob Gm, glob OW_PCVA} /\ 
+     (pk = OW_PCVA.sk.`1 /\ OW_PCVA.sk = sk){2} /\
+     (inv_G2_corr Gm.log RO.RO.m OW_PCVA.sk Gm.bad_corr Gm.m Gm.r){2}); last first.
+  + case: (Gm.bad_corr{1} <> None).
+    + inline *.
+      rcondf{2} 6; 1: by auto => /> /#.
+      swap{2} 5 8; sp; if{2}; auto => /> /#.
+    conseq (:true); 1: smt(). 
+    by do 2!( call{2}(:true ==> true); 1: by islossless); auto.
+  wp; call (: ={glob RO.RO, glob Gm, glob OW_PCVA} /\ 
+          (inv_G2_corr Gm.log RO.RO.m OW_PCVA.sk Gm.bad_corr Gm.m Gm.r){2}).
+  + proc; wp.
+    inline{1} 1; inline{2} 1.
+    sp 2 2; if => //; 2: by auto.
+    sp 2 2; elim * => rv_R rv_L.
+    if => //; 2: by auto => />; smt(findP_Some).
+    if => //; 1: by auto => />; smt(findP_Some).
+    if => //; auto => />; smt(findP_Some).
+  + proc; inline{1} 1; inline{2} 1; wp.
+    by ecall (G2_corr_H m{2}); wp; skip => /> /#. 
+  + by proc; wp; ecall (G2_corr_H x{2}).
+  inline *.
+  rcondt{1} ^if; 1: by auto => />; smt(mem_empty).
+  rcondt{2} ^if; 1: by auto => />; smt(mem_empty).
+  auto => />; smt(get_setE mem_empty).
+qed.
+
+local module G3 = {
+  import var OW_PCVA Gm O_AdvOW
+
+  module A = A(CountH(RO.RO), CountO(O_AdvOW))
+
+  proc main() : bool = {
+    var m' : plaintext;
+    var b;
+    RO.RO.init();
+    (pk, sk) <@ TT(RO.RO).kg();
+    m        <$ dplaintext;
+    r        <$ randd; 
+    cc       <- enc r pk m; 
+
+    CountO(O_AdvOW).init();
+    m'       <@ A.find(pk,cc);
+    b        <- dec sk.`2 cc = Some m' /\ m = m';
+    return b; 
+  }
+}.
+
+local equiv G2_G3_H : H(RO.RO).get ~ RO.RO.get : 
+  Gm.m{2} \notin RO.RO.m{2} /\
+  ={arg} /\ ={Gm.m, OW_PCVA.cc} /\
+     eq_except (pred1 Gm.m{2}) RO.RO.m{2} RO.RO.m{1} /\ OW_PCVA.sk{1}.`1 = O_AdvOW.pk{2} /\ RO.RO.m{2} = Gm.log{1} ==>
+  Gm.m{2} \notin RO.RO.m{2} =>
+  ={res} /\ ={Gm.m, OW_PCVA.cc} /\
+     eq_except (pred1 Gm.m{2}) RO.RO.m{2} RO.RO.m{1} /\ OW_PCVA.sk{1}.`1 = O_AdvOW.pk{2} /\ RO.RO.m{2} = Gm.log{1}.
+proof.
+  proc; inline *; wp; sp; if{1}; auto => />; smt(get_setE).
+qed.
+
+local lemma RO_in : phoare[RO.RO.get : Gm.m \in RO.RO.m ==> Gm.m \in RO.RO.m] =1%r.
+proof.
+  conseq (: true ==> true: = 1%r) (: Gm.m \in RO.RO.m ==> Gm.m \in RO.RO.m) => //.
+  + by proc; inline *; auto => />; smt(get_setE). 
+  by islossless.
+qed.
+
+(* This is magic ... *)
+local lemma G2_G3 &m : 
+  (forall (H0 <: POracle { -A }) (O <: VA_ORC { -A }),
+  islossless O.cvo => islossless O.pco => islossless H0.get => islossless A(H0, O).find) =>
+
+   Pr[G2.main() @ &m : res] <= 
+   Pr[G3.main() @ &m : res] + Pr[G3.main() @ &m : dec OW_PCVA.sk.`2 OW_PCVA.cc = Some Gm.m /\ Gm.m \in RO.RO.m].
+proof.
+  move => A_ll.
+  byequiv => //; proc; wp.
+  call (: Gm.m \in RO.RO.m, ={Gm.m, OW_PCVA.cc} /\ eq_except (pred1 Gm.m{2}) RO.RO.m{2} RO.RO.m{1} /\ 
+                   OW_PCVA.sk{1}.`1 = O_AdvOW.pk{2} /\ RO.RO.m{2} = Gm.log{1}).
+  + by proc; inline{1} 1; inline{2} 1; auto => />.
+  + by move=> *; islossless.
+  + by move=> *; conseq />; islossless.
+  + by proc; inline{1} 1; inline{2} 1; wp; call G2_G3_H; auto => /> /#.
+  + by move=> *; islossless.
+  + by move => /=; proc; inline 1; wp; call RO_in; auto.
+  + by proc; wp; call G2_G3_H; auto.
+  + by move=> *; islossless.
+  + by move=> *; proc; wp; call RO_in; auto.
+  inline *; auto => /> -[pk sk] hk m _ r _; smt(get_setE mem_empty).
+qed.
+
+local lemma G3_OW_CPA &m : 
+  Pr[G3.main() @ &m : res] <= 
+  Pr[OW_CPA(BasePKE, AdvOW(A)).main() @ &m : res].
+proof.
+  byequiv => //; proc.
+  inline{2} OW_CPA(BasePKE, AdvOW(A)).O.pco AdvOW(A).find BasePKE.dec; wp.
+  swap{2} 7 -6.
+  call (: ={glob RO.RO, OW_PCVA.cc, O_AdvOW.pk}); 1..3: by sim.  
+  inline *; auto.
+qed.
+
+local clone import PlugAndPray as PAP1 with
+  type tval <- int,
+  op indices <-  iota_ 0 (max 1 (qH + qP)), 
+  type tin <- unit, 
+  type tres <- bool
+  proof *.
+
+realize indices_not_nil by
+ smt(uniq_size_uniq iota_uniq size_iota size_eq0 ge0_qH ge0_qP).
+
+local equiv RO_count c : RO.RO.get ~ RO.RO.get : 
+  ={x, RO.RO.m} /\ card (fdom RO.RO.m{1}) = c ==>
+  ={res, RO.RO.m} /\ card (fdom RO.RO.m{1}) <= c + 1.
+proof.
+  proc; auto => /> &2 r; rewrite fdom_set fcardU fcard1; smt(fcard_ge0). 
+qed.
+
+local lemma G3_Adv_queryA :
+ (forall (RO<:POracle{ -CountO, -A })(O<:VA_ORC { -CountO, -A }), 
+  hoare [A(CountH(RO), CountO(O)).find : 
+       CountO.c_h = 0   /\ CountO.c_cvo = 0   /\ CountO.c_pco = 0 ==> 
+       CountO.c_h <= qH /\ CountO.c_cvo <= qV /\ CountO.c_pco <= qP]) =>
+
+  (forall (H0 <: POracle { -A }) (O <: VA_ORC { -A }),
+  islossless O.cvo => islossless O.pco => islossless H0.get => islossless A(H0, O).find) =>
+
+  equiv [
+  G3.A.find ~ AdvOW_query(A).A.find : 
+  ={arg} /\ ={glob A, OW_PCVA.cc, O_AdvOW.pk, RO.RO.m, glob CountO} /\ 
+    (CountO.c_h = 0   /\ CountO.c_cvo = 0   /\ CountO.c_pco = 0 /\ RO.RO.m = empty){1} ==> 
+  ={res} /\ ={glob A, OW_PCVA.cc, O_AdvOW.pk, RO.RO.m, glob CountO} /\
+    (CountO.c_h <= qH /\ CountO.c_cvo <= qV /\ CountO.c_pco <= qP /\
+    card (fdom RO.RO.m) <= qH + qP){1} ].
+proof.
+  move => A_count A_ll.
+  conseq (: ={arg} /\ ={glob A, OW_PCVA.cc, O_AdvOW.pk, RO.RO.m, glob CountO} /\ 
+           (card (fdom RO.RO.m) <= CountO.c_h + CountO.c_pco){1} ==> 
+            ={res} /\ ={glob A, OW_PCVA.cc, O_AdvOW.pk, RO.RO.m, glob CountO} /\ 
+            (card (fdom RO.RO.m) <= CountO.c_h + CountO.c_pco){1})
+         (A_count (<:RO.RO) (<:O_AdvOW)) => />.
+  + by rewrite fdom0 fcards0. + smt().
+  proc ( ={OW_PCVA.cc, O_AdvOW.pk, RO.RO.m, glob CountO} /\ 
+            (card (fdom RO.RO.m) <= CountO.c_h + CountO.c_pco){1}) => //.
+  + conseq />; sim.
+  + by proc; inline {1} 1; inline {2} 1; wp; ecall (RO_count (card (fdom RO.RO.m{1}))); auto => /> /#.
+  proc; wp;  ecall (RO_count (card (fdom RO.RO.m{1}))); auto => /> /#.
+qed.
+
+local lemma count0 :
+ qH = 0 => qP = 0 =>
+ (forall (RO<:POracle{ -CountO, -A })(O<:VA_ORC { -CountO, -A }), 
+  hoare [A(CountH(RO), CountO(O)).find : 
+       CountO.c_h = 0   /\ CountO.c_cvo = 0   /\ CountO.c_pco = 0 ==> 
+       CountO.c_h <= qH /\ CountO.c_cvo <= qV /\ CountO.c_pco <= qP]) =>
+
+hoare [
+  G3.A.find : 
+  CountO.c_h = 0 /\ CountO.c_pco = 0 /\ CountO.c_cvo = 0 /\ RO.RO.m = empty==>
+  RO.RO.m = empty].
+proof.
+move => qH0 qP0 A_count.
+conseq (:card (fdom RO.RO.m) <= CountO.c_h + CountO.c_pco  ==>
+         card (fdom RO.RO.m) <= CountO.c_h + CountO.c_pco) 
+                (A_count  (<:RO.RO) (<:O_AdvOW));1,2:
+                 smt(fdom0 fcards0 fdom_eq0 fcard_ge0 fcard_eq0).
+proc (card (fdom RO.RO.m) <= CountO.c_h + CountO.c_pco);
+       1,2:smt(fdom0 fcards0 fdom_eq0 fcard_ge0 fcard_eq0).
+
++ by proc;wp;call(:card (fdom RO.RO.m) <= CountO.c_h + CountO.c_pco);auto. 
++ proc; wp;call(_:card (fdom RO.RO.m) <= CountO.c_h + CountO.c_pco ==>
+                   card (fdom RO.RO.m) <= CountO.c_h + CountO.c_pco + 1).
+  + by proc;inline *; auto; move => &hr ? r _ /=;smt(card_set).   
+  by auto;smt(fdom0 fcards0 fdom_eq0 fcard_ge0 fcard_eq0).
++ proc; wp. call(_:card (fdom RO.RO.m) <= CountO.c_h + CountO.c_pco ==>
+                   card (fdom RO.RO.m) <= CountO.c_h + CountO.c_pco + 1).
+  proc;inline *; auto.  move => &hr ? r _ /=; smt(card_set). 
+   by auto;smt(fdom0 fcards0 fdom_eq0 fcard_ge0 fcard_eq0).
+qed.
+
+local lemma G3_OW_CPA_query &m : 
+ (forall (RO<:POracle{ -CountO, -A })(O<:VA_ORC { -CountO, -A }), 
+  hoare [A(CountH(RO), CountO(O)).find : 
+       CountO.c_h = 0   /\ CountO.c_cvo = 0   /\ CountO.c_pco = 0 ==> 
+       CountO.c_h <= qH /\ CountO.c_cvo <= qV /\ CountO.c_pco <= qP]) =>
+
+  (forall (H0 <: POracle { -A }) (O <: VA_ORC { -A }),
+  islossless O.cvo => islossless O.pco => islossless H0.get => islossless A(H0, O).find) =>
+
+  Pr[G3.main() @ &m : dec OW_PCVA.sk.`2 OW_PCVA.cc = Some Gm.m /\ Gm.m \in RO.RO.m] <=
+  (qH + qP)%r * Pr[OW_CPA(BasePKE, AdvOW_query(A)).main() @ &m : res].
+proof.
+  move => A_count A_ll.
+  case (qH = 0 /\ qP = 0). 
+  + move => [#] qH0 qP0; rewrite qH0 qP0 /=.
+    byphoare => //;hoare.
+    conseq (_: _ ==> RO.RO.m = empty); 1: by smt(mem_empty).
+    proc;wp;seq 6 : (CountO.c_h = 0 /\ CountO.c_pco = 0 /\ CountO.c_cvo = 0 /\
+                      RO.RO.m = empty); 1: by inline*;auto.
+    by call count0.
+       
+  move => qHPn0.
+  rewrite RField.mulrC -StdOrder.RealOrder.ler_pdivr_mulr; 1: smt (ge0_qH ge0_qP).
+print glob G3.
+  pose phi := fun (g:glob G3) (b:bool) => dec g.`7.`2 g.`8 = Some g.`2 /\ g.`2 \in g.`9.
+  pose psi := fun (g:glob G3) (_:bool) => 
+    let i = find (pred1 g.`2) (elems (fdom g.`9)) in
+    if 0 <= i < qH + qP then i else 0.
+  have := PAP1.PBound G3 phi psi tt &m _. 
+  + smt (ge0_qH ge0_qP mem_iota).
+  rewrite undup_id 1:iota_uniq size_iota.
+  have -> : max 0 (max 1 (qH  + qP)) = qH + qP by smt (ge0_qH ge0_qP).
+  rewrite (RField.mulrC (1%r/_)) RField.mulrA /= => ->.
+  byequiv => //; rewrite /phi /psi /=.
+  proc.
+  inline{2} 5; inline{2} 8; inline{2} 4; wp; rnd.
+  inline{2} 6; inline{1} 1; wp.
+  call G3_Adv_queryA; inline *; auto => />.
+  move=> [pk sk] hpk m hm r hr c_cvo c_h c_pco ro 3?.
+  rewrite cardE => hs. 
+  have -> /= : max 1 (qH + qP) = qH + qP; 1: by smt(ge0_qH ge0_qP).
+  split; 1: by smt().
+  move  => /> _ i _ _ -> hin ->>.
+  have -> /= : 0 <= find (pred1 m) (elems (fdom ro)) && find (pred1 m) (elems (fdom ro)) < qH + qP.
+  + rewrite find_ge0.
+    have := has_find (pred1 m) (elems (fdom ro)).
+    by rewrite has_pred1 -memE mem_fdom hin /= /#.
+  have := nth_find witness (pred1 m) (elems (fdom ro)).
+  rewrite {2}/pred1 => -> //.
+  by rewrite has_pred1 -memE mem_fdom hin.
+qed.
+
+lemma corr_red_count (RO <: RO.RO {-CountO, -A, -CO1, -Gm, -OW_PCVA}):
+ (forall (RO<:POracle{ -CountO, -A })(O<:VA_ORC { -CountO, -A }), 
+  hoare [A(CountH(RO), CountO(O)).find : 
+       CountO.c_h = 0   /\ CountO.c_cvo = 0   /\ CountO.c_pco = 0    ==> 
+       CountO.c_h <= qH /\ CountO.c_cvo <= qV /\ CountO.c_pco <= qP]) =>
+ hoare [
+   AdvCorr(A, CO1(RO)).A.find : CO1.counter = 1 /\ CountO.c_h = 0 /\ CountO.c_cvo = 0 /\
+       CountO.c_pco = 0 ==> CO1.counter <= 1 + qH + qP].
+move => A_count.
+conseq(:CO1.counter <= CountO.c_pco + CountO.c_h + 1 ==> CO1.counter <= CountO.c_pco + CountO.c_h + 1) 
+   (A_count (H(CO1(RO))) (G2_O(CO1(RO)))); 1,2: smt().
++ proc(CO1.counter <= CountO.c_pco + CountO.c_h + 1);1,2:smt().
++ by proc;inline *;auto => />.
++ proc;inline *;sp;if;last by auto => /#.
+  sp;if;sp;if; 1: by wp;call(_: true);auto => /#.
+  by wp;call(_: true);auto => /#.
+  by wp;call(_: true);auto => /#.
+  by auto => /#.
++ proc;inline *;sp;if;last by auto => /#.
+  sp;if;sp;if; 1: by wp;call(_: true);auto => /#.
+  by wp;call(_: true);auto => /#.
+  by wp;call(_: true);auto => /#.
+  by auto => /#.
+qed.
+
+lemma pre_conclusion &m gamma_spread :
+ gamma_spread_ok gamma_spread =>
+
+ (forall (RO<:POracle{ -CountO, -A })(O<:VA_ORC { -CountO, -A }), 
+  hoare [A(CountH(RO), CountO(O)).find : 
+       CountO.c_h = 0   /\ CountO.c_cvo = 0   /\ CountO.c_pco = 0  ==> 
+       CountO.c_h <= qH /\ CountO.c_cvo <= qV /\ CountO.c_pco <= qP]) =>
+
+  (forall (H0 <: POracle { -A }) (O <: VA_ORC { -A }),
+  islossless O.cvo => islossless O.pco => islossless H0.get => islossless A(H0, O).find) =>
+
+  Pr[OW_PCVA(RO.LRO, TT, A).main() @ &m : res] <=
+      Pr[OW_CPA(BasePKE, AdvOW(A)).main() @ &m : res]
+    + (qH + qP)%r * Pr[OW_CPA(BasePKE, AdvOW_query(A)).main() @ &m : res]
+    + Pr[ Correctness_Adv(RO.RO,TT,AdvCorr(A)).main() @ &m : res ]
+    + qV%r * gamma_spread.
+proof.
+  move => gs_ok A_count A_ll.
+  by move: (OW_PCVA_gamma &m gamma_spread gs_ok A_count A_ll) (G1_G2 &m A_ll) (G2_correctness &m) (G2_G3 &m  A_ll)
+     (G3_OW_CPA &m) (G3_OW_CPA_query &m  A_count A_ll) => /#.
+qed.
+
+(* +2 could be reduced to +1 because we know the message
+   output by our adv is always in the ROM table.
+   +1 comes from the pre-fetch of Gm.r. *)
+
+lemma conclusion &m gamma_spread :
+ qH + qP + 1 = qHC =>
+
+ qHC < FinT.card -1 =>
+
+ gamma_spread_ok gamma_spread =>
+
+ (forall (RO<:POracle{ -CountO, -A })(O<:VA_ORC {-CountO, -A}), 
+  hoare [A(CountH(RO), CountO(O)).find : 
+       CountO.c_h = 0   /\ CountO.c_cvo = 0   /\ CountO.c_pco = 0 ==> 
+       CountO.c_h <= qH /\ CountO.c_cvo <= qV /\ CountO.c_pco <= qP]) =>
+
+  (forall (H0 <: POracle { -A }) (O <: VA_ORC { -A }),
+  islossless O.cvo => islossless O.pco => islossless H0.get => islossless A(H0, O).find) =>
+
+  Pr[OW_PCVA(RO.LRO, TT, A).main() @ &m : res] <=
+      Pr[OW_CPA(BasePKE, AdvOW(A)).main() @ &m : res]
+    + (qH + qP)%r * Pr[OW_CPA(BasePKE, AdvOW_query(A)).main() @ &m : res]
+    + (qH + qP + 2)%r * Pr[ PKE.Correctness_Adv(BasePKE,B(AdvCorr(A),RO.LRO)).main() @ &m : res ]
+    + qV%r * gamma_spread.
+proof.
+  move => counts qhc_small gs_ok A_count A_ll.
+  move: (pre_conclusion &m gamma_spread gs_ok A_count A_ll).
+  move: (correctness (AdvCorr(A)) &m qhc_small _ _). 
+  + move => RO; proc;wp.
+    call (corr_red_count RO).
+    inline *;wp;conseq />.
+    seq 6 : #pre; 1: by auto.
+    if;if. 
+    + wp;call(_:true);auto => /#.
+    + wp;call(_:true);auto => /#.
+    + wp;call(_:true);auto => /#.
+    auto => /#.
+  move => H0 H0_ll;proc;inline *;wp.
+  by call(_: true); islossless. 
+  by smt().
+qed.
+
+(* Benjamin's original notes.
+(* Final lemma will be *)
+lemma conclusion &m :
+  Pr[OW_PCVA(RO.RO, TT, A).main() @ &m : res] <=
+      Pr[OW_CPA(BasePKE, AdvOW(A)).main() @ &m : res]
+    + (qH + qP)%r * Pr[OW_CPA(BasePKE, AdvOW_query(A)).main() @ &m : res]
+    + (qH + qP) %r * Pr[ Correctness_Adv(BasePKE,AdvCorr(A)).main() @ &m : res ]
+    + qV%r * gamma_spread.
+
+(* I think we can proof that *) 
+lemma conclusion &m :
+  Pr[OW_PCVA(RO.RO, TT, A).main() @ &m : res] <=
+      Pr[OW_CPA(BasePKE, AdvOW(A)).main() @ &m : res]
+    + (qH)%r * Pr[OW_CPA(BasePKE, AdvOW_query(A)).main() @ &m : res]
+    + (qH) %r * Pr[ Correctness_Adv(BasePKE,AdvCorr(A)).main() @ &m : res ]
+    + (qV + qP)%r * gamma_spread.
+*)
+
+end section.
+*)
